Derive a circuit

gol_gatesScript.sml
@@ -149,5 +149,59 @@ val _ = translate_gate [0,1,2,3] half_adder_ee_es;
 val _ = translate_gate [0,1,2,3] half_adder_ee_ee;
 val _ = translate_gate [2] slow_wire_e_e;
 
+Definition delay_def:
+  delay n a i = if i < n then F else a (i - n:num)
+End
+
+Definition conj_def:
+  conj a b = (λn. a n ∧ b n)
+End
+
+Definition disj_def:
+  disj a b = (λn. a n ∨ b n)
+End
+
+Definition set_env_def:
+  set_env a b (A,n) = a n ∧
+  set_env a b (B,n) = b n
+End
+
+Theorem delay_simp:
+  (λn. delay k a (k + n)) = a ∧
+  (λn. delay k a (n + k)) = a
+Proof
+  gvs [FUN_EQ_THM,delay_def]
+QED
+
+Theorem simulation_ok_2:
+  simulation_ok w h [((x1,x2),d,Var A a_d); ((x1',x2'),d',Var B b_d)] outs init ⇒
+  ∀a b.
+    circuit
+      (make_area w h)
+      [((x1,x2),d,a); ((x1',x2'),d',b)]
+      (eval_io (set_env (delay a_d a) (delay b_d b)) outs) []
+      (from_rows (-85,-85)
+        (MAP (MAP (eval (set_env (delay a_d a) (delay b_d b)))) init))
+Proof
+  rw []
+  \\ drule simulation_ok_IMP_circuit
+  \\ disch_then $ qspec_then ‘(set_env (delay a_d a) (delay b_d b))’ mp_tac
+  \\ gvs [eval_io_def,set_env_def,delay_simp]
+QED
+
+fun make_abbrev name tm =
+  let
+    val v = mk_var(name,type_of tm)
+    val th = new_definition(name,mk_eq(v,tm))
+  in SYM th end
+
+Theorem and_en_e_circuit =
+  MATCH_MP simulation_ok_2 (theorem "and_en_e_thm")
+  |> CONV_RULE ((QUANT_CONV o QUANT_CONV o RAND_CONV o RAND_CONV)
+       (REWRITE_CONV [definition "and_en_e_def"] THENC EVAL
+        THENC make_abbrev "and_en_e_concrete"))
+  |> SRULE [eval_io_def,set_env_def,GSYM conj_def,GSYM disj_def,
+            SF ETA_ss, make_area_def];
+
 val _ = (max_print_depth := 10); (* avoids blow up in size of Theory.sig file *)
 val _ = export_theory();
